CertifyingDatalog/Database.lean
@@ -1,8 +1,11 @@
 import CertifyingDatalog.Datalog
 
-instance mockDatabase (τ: signature) [DecidableEq τ.vars] [DecidableEq τ.constants] [DecidableEq τ.relationSymbols]: database τ where
+instance mockDatabase (τ: signature) [DecidableEq τ.vars] [DecidableEq τ.constants] [DecidableEq τ.relationSymbols] [Hashable τ.constants] [Hashable τ.vars] [Hashable τ.relationSymbols]
+: database τ where
   contains:= fun _ => true
 
-def mockDatabaseContainedInModel {τ: signature} [DecidableEq τ.vars] [DecidableEq τ.constants] [DecidableEq τ.relationSymbols] (d: database τ) (i: Set (groundAtom τ)): Bool := true
+def mockDatabaseContainedInModel {τ: signature} [DecidableEq τ.vars] [DecidableEq τ.constants] [DecidableEq τ.relationSymbols] [Hashable τ.constants] [Hashable τ.vars] [Hashable τ.relationSymbols]
+ (d: database τ) (i: Set (groundAtom τ)): Bool := true
 
-axiom mockDatabaseContainedInModelTrue {τ: signature} [DecidableEq τ.vars] [DecidableEq τ.constants] [DecidableEq τ.relationSymbols] (d: database τ) (i: Set (groundAtom τ)): mockDatabaseContainedInModel d i = true ↔ ∀ (ga: groundAtom τ), d.contains ga → ga ∈ i
+axiom mockDatabaseContainedInModelTrue {τ: signature} [DecidableEq τ.vars] [DecidableEq τ.constants] [DecidableEq τ.relationSymbols] [Hashable τ.constants] [Hashable τ.vars] [Hashable τ.relationSymbols]
+ (d: database τ) (i: Set (groundAtom τ)): mockDatabaseContainedInModel d i = true ↔ ∀ (ga: groundAtom τ), d.contains ga → ga ∈ i
