CertifyingDatalog/ModelChecking.lean
@@ -4,15 +4,15 @@ import CertifyingDatalog.Unification
 import Mathlib.Data.Set.Basic
 import CertifyingDatalog.Basic
 
-structure partialGroundRule (τ: signature)[DecidableEq τ.vars] [DecidableEq τ.constants] [DecidableEq τ.relationSymbols] [Inhabited τ.constants] (i: interpretation τ) where
+structure partialGroundRule (τ: signature)[DecidableEq τ.vars] [DecidableEq τ.constants] [DecidableEq τ.relationSymbols] [Inhabited τ.constants] [Hashable τ.constants] [Hashable τ.relationSymbols] [Hashable τ.vars] (i: interpretation τ) where
   head: atom τ
   groundedBody: List (groundAtom τ)
   ungroundedBody: List (atom τ)
 
   members: ∀ (ga: groundAtom τ), ga ∈ groundedBody → ga ∈ i
 
-variable  {τ: signature}[DecidableEq τ.vars] [DecidableEq τ.constants] [DecidableEq τ.relationSymbols] [Inhabited τ.constants] {i: interpretation τ}
-
+variable  {τ: signature}[DecidableEq τ.vars] [DecidableEq τ.constants] [DecidableEq τ.relationSymbols] [Inhabited τ.constants]  [Hashable τ.constants] [Hashable τ.vars] [Hashable τ.relationSymbols]
+ {i: interpretation τ}
 def partialGroundRule.isSafe (pgr: partialGroundRule τ i): Prop :=
   atomVariables pgr.head ⊆ collectResultsToFinset atomVariables pgr.ungroundedBody
 
